Veritas.SeqOps.fst
@@ -1,0 +1,66 @@
+module Veritas.SeqOps 
+
+let rec interleave_map_aux (#a:eqtype) 
+                   (#p:pos) 
+                   (s:seq a) 
+                   (ss: seq (seq a){length ss = p}) 
+                   (prf: interleave #a #p s ss)
+                   (i:seq_index s): 
+  Tot (j:(nat*nat){fst j < p /\ 
+            snd j < length (index ss (fst j)) /\
+            index (index ss (fst j)) (snd j) = index s i} )
+  (decreases prf)
+            = 
+  match prf with
+  | IntEmpty -> assert(s == empty #a); (0,0)
+  | IntAdd s' ss' prf' x i' -> if i = length s' then 
+                                 (i', length (index ss' i'))                               
+                               else
+                                 interleave_map_aux s' ss' prf' i
+
+let interleave_map (#a:eqtype) 
+                   (#p:pos) 
+                   (s:seq a) 
+                   (ss: seq (seq a){length ss = p}) 
+                   (prf: interleave #a #p s ss)
+                   (i:seq_index s): 
+  Tot (j:(nat*nat){fst j < p /\ 
+            snd j < length (index ss (fst j)) /\
+            index (index ss (fst j)) (snd j) = index s i} ) = 
+  interleave_map_aux s ss prf i
+
+let rec interleave_inv_map_aux (#a:eqtype)
+                       (#p:pos)
+                       (s:seq a)
+                       (ss: seq (seq a){length ss = p})
+                       (prf:interleave #a #p s ss)
+                       (j:(nat*nat){fst j < p /\ 
+                                  snd j < length (index ss (fst j))}): 
+  Tot (i:(seq_index s){index (index ss (fst j)) (snd j) = index s i}) 
+  (decreases prf)
+  = 
+  match prf with
+  | IntEmpty -> 0
+  | IntAdd s' ss' prf' x i' -> let p,q = j in
+                               let si' = index ss' i' in
+                               if p = i' && q = length si' then
+                                 length s'
+                               else
+                                 interleave_inv_map_aux s' ss' prf' j
+
+let interleave_inv_map (#a:eqtype)
+                       (#p:pos)
+                       (s:seq a)
+                       (ss: seq (seq a){length ss = p})
+                       (prf:interleave #a #p s ss)
+                       (j:(nat*nat){fst j < p /\ 
+                                  snd j < length (index ss (fst j))}): 
+  Tot (i:(seq_index s){index (index ss (fst j)) (snd j) = index s i}) = 
+  interleave_inv_map_aux s ss prf j
+
+let partition_aux (#a:eqtype) (#p:pos) (s:seq a) (pf: a -> (i:nat{i < p})): 
+  ss:seq (seq a){length ss = p /\ interleave #a #p s ss} = admit()
+
+(* partition a sequence into independent sequences based on a partition function pf *)
+let partition (#a:eqtype) (#p:pos) (s:seq a) (pf: a -> (i:nat{i < p})): 
+  ss:seq (seq a){length ss = p /\ interleave #a #p s ss} = partition_aux #a #p s pf
