Veritas.Verifier.Correctness.fst
@@ -6,6 +6,7 @@ open Veritas.MultiSetHash
 open Veritas.Record
 open Veritas.Verifier
 open Veritas.SeqAux
+open Veritas.SeqOps
 
 //Allow the solver to unroll recursive functions at most once (fuel)
 //Allow the solver to invert inductive definitions at most once (ifuel)
@@ -34,61 +35,5 @@ let vprefix (#p:pos) (l:verifiable_log #p) (i:nat{i <= length l}):
   lemma_verifiable_implies_prefix_verifiable l i;
   prefix l i
 
-(* is this a thread-local operation *)
-let is_thread_op (e:vlog_entry_g) = TOp? e
 
-(* is the operator at index i a thread-local op *)
-let is_thread_op_idx (l:vlog) (i:vl_index l) = 
-  is_thread_op (index l i)
-
-(* thread id of a thread-local op *)
-let thread_id_of (e:vlog_entry_g {is_thread_op e}) = 
-  TOp?.tid e
-
-let thread_id_of_idx (l:vlog) (i:vl_index l{is_thread_op_idx l i}) = 
-  thread_id_of (index l i)
-
-(* thread id of every thread-local op < p (verifier parallelism) *)
-let lemma_thread_id_valid (#p:pos) 
-                          (l:verifiable_log #p) 
-                          (i:vl_index l {is_thread_op_idx l i})
-  : Lemma (thread_id_of_idx l i < p) = 
-  let l' = vprefix l i in
-  let l'' = vprefix l (i + 1) in
-  ()
-         
-(* 
- * we associate a timestamp to every thread-local op based on the 
- * thread clock after the completion of the operation 
- *)
-let op_clock (#p:pos) 
-             (l:verifiable_log #p) 
-             (i:vl_index l {is_thread_op_idx l i}): timestamp = 
- let l' = vprefix l (i + 1) in
- let vs = verifier #p l' in
- let ti = thread_id_of_idx l i in
- lemma_thread_id_valid l i;
- thread_clock ti vs
-
-(* thread-local log: a log with only thread-local operations (no VerifyEpoch) *)
-type thread_local_log (l:vlog) = forall (i:vl_index l). {:pattern (is_thread_op_idx l i)} is_thread_op_idx l i
-
-type tl_log (#p:pos) = l:(verifiable_log #p){thread_local_log l}
-
-(* a thread-local log is clock-ordered is the clock of each operation is monotonically increasing *)
-type clock_ordered_log (#p:pos) (l:tl_log #p) = 
-  forall (i:vl_index l). i > 0 ==> (op_clock l i `ts_geq` op_clock l (i - 1))
-
-type co_log (#p:pos) = l:(tl_log #p){clock_ordered_log l}
-
-(* the key referenced by an log operation *)
-let key_of (e:vlog_entry) = 
-  match e with
-  | Get k _ -> k
-  | Put k _ -> k
-  | AddM r _ -> let (k,_) = r in k
-  | EvictM k _ -> k
-  | AddB r _ _ -> let (k,_) = r in k
-  | EvictB k _ -> k
-  | EvictBM k _ _ -> k
 
